theories/run_prop.v
@@ -1,20 +1,21 @@
 From mathcomp Require Import all_ssreflect.
 From det Require Import run.
+Import Language.
 
-Module RunP (A: Unif).
-  Module Run := Run(A).
-  Import Run Language.
+Section RunP.
+  Variable u: Unif.
+  (* Notation *)
 
   Lemma expanded_classic_expanded {s A r}:
-    Run.expanded_classic s A r -> Run.expanded s A r.
+    expanded_classic u s A r -> expanded u s A r.
   Proof. by exists false. Qed.
   
   Lemma run_classic_run {s A s1 B}:
-    run_classic s A s1 B -> run s A s1 B.
+    run_classic u s A s1 B -> run u s A s1 B.
   Proof. by exists false. Qed.
 
   Lemma run_classic_cut {s s2 A B s3 C}:
-    run_classic s A s3 C -> expand s A = CutBrothers s2 B -> False.
+    run_classic u s A s3 C -> expand u s A = CutBrothers s2 B -> False.
   Proof.
     rewrite /run_classic; remember false as f eqn:Hf => H.
     elim: H s2 B Hf; clear.
@@ -25,13 +26,13 @@ Module RunP (A: Unif).
   Qed.
 
   Lemma run_Solved_id {s s1 A r alt}:
-      expand s A = Success s1 alt -> expanded s A r -> r = Done s1 alt.
+      expand u s A = Success s1 alt -> expanded u s A r -> r = Done s1 alt.
   Proof.
     move=> + [b H]; by case: H => //=; clear; congruence.
   Qed.
 
   Lemma expanded_consistent: forall {s0 A s1 s2 b1 b2},
-    expandedb s0 A s1 b1 -> expandedb s0 A s2 b2 -> s1 = s2 /\ b1 = b2.
+    expandedb u s0 A s1 b1 -> expandedb u s0 A s2 b2 -> ((s1 = s2) * (b1 = b2))%type.
   Proof.
     move=> s0 A s1 + b1 + H.
     elim:H; clear.
@@ -40,263 +41,174 @@ Module RunP (A: Unif).
       by inversion H1; try congruence; subst.
     + move=> s A B HA r b H0.
       inversion H0; try congruence; subst.
-      by move: H1; rewrite HA => -[] /[subst1].
+      move: H; rewrite HA => -[] /[subst1]//.
     + move=> s1 s2 r A B b HA HB IH s3 b1; inversion 1; try congruence; subst.
-      move: H1; rewrite HA => -[] /[subst2].
-      by have:= IH _ _ H2 => -[] /[subst2].
+      move: H0; rewrite HA => -[] /[subst2].
+      by have:= IH _ _ H1 => -[] /[subst2].
     + move=> s1 s2 r A B b1 + HB IH r2 b2 HA.
-      by inversion HA; try congruence; subst; rewrite H0 => -[] /[subst2]; auto.
+      by inversion HA; try congruence; subst; rewrite H => -[] /[subst2]; auto.
   Qed.
 
   Lemma run_consistent {s A s1 B b1}:
-    runb s A s1 B b1 -> forall {s2 C b2}, runb s A s2 C b2 -> s1 = s2 /\ B = C /\ b1 = b2.
+    runb u s A s1 B b1 -> forall {s2 C b2}, runb u s A s2 C b2 -> ((s1 = s2) * (B = C) * (b1 = b2))%type.
   Proof.
     move=> H; elim: H; clear.
     + move=> s s' A B C b H -> s2 D b2 H1.
       inversion H1; clear H1; subst;
         by have:= expanded_consistent H H0 => -[] // [->->]->.
-    (* + move=> s A B b HA HB r b2 H1.
-      inversion H1; clear H1; subst => //; have []:= expanded_consistent HA H0; try congruence.
-      by move=> [_ <-]. *)
     + move=> s s1 s2 A B C D b1 b2 b3 HA HB HC IH ? s3 E s4 H1; subst.
-      inversion H1; subst; have [] := expanded_consistent HA H0 => //.
+      inversion H1; subst; have [] := expanded_consistent HA H => //.
       move=>[??]; subst.
-      move: H2; rewrite HB => -[??]; subst.
-      by have:= IH _ _ _ H3 => -[?[??]]; subst.
+      move: H0; rewrite HB => -[??]; subst.
+      have {}H := IH _ _ _ H2.
+      rewrite !H//.
   Qed.
 
-  Lemma expand_solved_expand {s s1 s2 s3 A B C}: 
-    expand s A = Success s2 B -> expanded s1 B (Done s3 C) -> B = C /\ s1 = s3.
+  Lemma ges_subst_cutl {s A} : get_substS s (cutl A) = get_substS s A.
   Proof.
-    move=>/expand_solved_success[_ sB][v].
-    move=>/expanded_success => /(_ sB)[][]//.
+    elim: A s => //=.
+    - move=> A HA s B HB s1; case:ifP => //=dA; rewrite ?is_dead_cutl dA//.
+    - move=> A HA B0 _ B HB s; case:ifP; rewrite success_cut => sA; rewrite sA HA//.
   Qed.
 
-  Section same_structure.
-
-    Fixpoint same_structure A B :=
-      match A with
-      | And A1 B0 B1 =>
-        match B with 
-        | And A' B0' B' => [&& same_structure B0 B0', same_structure A1 A' & same_structure B1 B']
-        | _ => false
-        end
-      | Or A1 s B1 =>
-        match B with 
-        | Or A' s' B' => [&& s == s', same_structure A1 A' & same_structure B1 B']
-        | _ => false
-        end
-      | _ => true
-      end.
-
-    Lemma same_structure_id {A}: same_structure A A.
-    Proof. 
-      elim: A => //=.
-        by move=>?->??->; rewrite eqxx.
-      by move=> ?->? ->?->.
-    Qed.
-
-    Lemma same_structure_trans: transitive same_structure.
-    Proof.
-      move=> + A; elim: A => //.
-      - move=> A HA s B HB []//A' s' B'[]//A2 s2 B2/=.
-        move=>/and3P[/eqP<-HA' HB']/and3P[/eqP<-HA2 HB2].
-        rewrite eqxx (HA A' A2)//(HB B' B2)//.
-      - move=> A HA B0 HB0 B HB[]//A1 B01 B1[]//A2 B02 B2/=.
-        move=>/and3P[HA1 HB01 HB1]/and3P[HA2 HB02 HB2].
-        rewrite (HA A1 A2)//(HB B1 B2)//(HB0 B01 B02)//.
-    Qed.
-
-    Lemma same_structure_cutr {A B}: same_structure A B -> same_structure A (cutr B).
-    Proof. 
-      elim: A B => //=.
-        by move=> A HA s B HB []// A' s' B' /= /and3P[/eqP<-/HA->/HB->]; rewrite eqxx.
-      move=> A HA B0 HB0 B HB []//A' B0' B'/=/and3P[/HB0-> /HA-> /HB->]//.
-    Qed.
-    
-    Lemma same_structure_cut {A B}: same_structure A B -> same_structure A (cutl B).
-    Proof. 
-      elim: A B => //=.
-        move=> A HA s B HB []// A' s' B' /= /and3P[/eqP<- H2 H3].
-        case: ifP => //.
-          by rewrite H2 HB//eqxx.
-        by rewrite eqxx HA// same_structure_cutr//.
-      move=> A HA B0 HB0 B HB []//A' B0' B'/=. 
-      move=> /and3P[sB0 sA sB].
-      rewrite HA//HB0//HB//.
-    Qed.
-    
-    Lemma same_structure_dead {B}: same_structure B (dead1 B).
-    Proof. 
-      elim: B => //=.
-        move=> A HA s B HB; rewrite eqxx HA HB//.
-      move=> A HA B0 HB0 B HB; rewrite HA HB0 HB//.
-    Qed.
-
-    Lemma expand_same_structure {s A r}: 
-      expand s A = r -> same_structure A (get_state r).
-    Proof.
-      elim: A s r => //.
-        move=> A HA s B HB s1 [s2|s2||s2] C.
-        - move=> /=.
-          case: ifP => dA.
-            case eB: expand => //[s1' B'|s1' B'][_<-]; rewrite eqxx same_structure_id (HB _ _ eB)//.
-          case eA: expand => //[s1' A'|s1' A'][_<-]; rewrite eqxx (HA _ _ eA)?same_structure_id// same_structure_cutr//same_structure_id//.
-        - move=> /=; case: ifP => dA; case: expand => //.
-        - move=> /simpl_expand_or_fail [].
-            by move=>[A'[_[HA'->]]]/=; rewrite eqxx (HA _ _ HA') same_structure_id.
-          by move=> [B'[_ [HB'->]]]/=; rewrite eqxx same_structure_id (HB _ _ HB').
-        - move=> /simpl_expand_or_solved[].
-            by move=>[A'[HA'->]]/=; rewrite eqxx same_structure_id (HA _ _ HA').
-          by move=> [B'[_ [HB'->]]]/=; rewrite eqxx same_structure_id (HB _ _ HB').
-      move=> A HA B0 HB0 B HB s1 [s2|s2||s2]C.
-      - move=> /simpl_expand_and_expanded[].
-          by move=>[A'[HA'->]]/=; rewrite !same_structure_id (HA _ _ HA').
-        by move=> [s'[A'[B' [HA'[HB' ->]]]]]/=; rewrite (HA _ _ HA') (HB _ _ HB') same_structure_id.
-      - move=> /simpl_expand_and_cut[].
-          by move=>[A'[HA'->]]/=; rewrite !same_structure_id (HA _ _ HA').
-        move=>[s'[A'[B'[HA'[HB' ->]]]]]/=; rewrite (HB _ _ HB')//(same_structure_cut same_structure_id).
-        by have:= (HA _ _ HA') => /same_structure_cut->.
-      - move=> /simpl_expand_and_fail[].
-          by move=> [A'[HA'->]]/=; rewrite !same_structure_id (HA _ _ HA').
-        by move=> [s'[A'[B'[HA'[HB' ->]]]]]/=; rewrite (HA _ _ HA') (HB _ _ HB') same_structure_id.
-      - by move=> /simpl_expand_and_solved [s'[A'[B'[HA'[HB'->]]]]]/=; rewrite (HA _ _ HA') (HB _ _ HB') same_structure_id.
-    Qed.
-
-    Lemma expandedb_same_structure {s A r b}: 
-      expandedb s A r b -> same_structure A (get_state_exp r).
-    Proof.
-      move=> H; elim: H; clear => /=.
-      + move=> s1 s2 A B.
-        apply: expand_same_structure.
-      + move=> ???; apply: expand_same_structure.
-      + move=> ??????/expand_same_structure/= + _.
-        apply: same_structure_trans.
-      + move=> ??????/expand_same_structure/= + _.
-        apply: same_structure_trans.
-    Qed.
-
-    Lemma same_structure_clean_success {A}:
-      same_structure A (clean_success A).
-    Proof.
-      elim: A => //.
-      - move=> A HA s B HB/=; case: ifP => //_; rewrite ?HA?HB same_structure_id eqxx//.
-      - move=> A HA B0 _ B HB/=; case: ifP => _; rewrite !same_structure_id//?HA//.
-    Qed.
-  End same_structure.
-  
+  (* Lemma ges_subst_3 {s A B} :
+    success A -> get_substS (get_substS (get_substS s A) B) A = get_substS (get_substS s A) B.
+  Proof.
+    elim: A s B => //=.
+    - move=> A HA s B HB s1 C; case: ifP => //dA. rewrite dA//.
+    - move=> A HA B0 _ B HB s1 C; case: ifP => sA; rewrite sA//.
+      rewrite -HB.
+    elim: A s => //=.
+    - move=> A HA s B HB s1; case:ifP => //=dA; rewrite ?is_dead_cutl dA//.
+    - move=> A HA B0 _ B HB s; case:ifP; rewrite success_cut => sA; rewrite sA HA//.
+  Qed. *)
 
   Lemma expanded_and_complete {s s' C A B0 B b} :
-    expandedb s (And A B0 B) (Done s' C) b ->
-      exists s'' A' B' b1 b2, expandedb s A (Done s'' A') b1 /\ expandedb s'' B (Done s' B') b2 /\ b = b1 || b2.
+    expandedb u s (And A B0 B) (Done s' C) b ->
+      exists s'' A' B' b1 b2, expandedb u s A (Done s'' A') b1 /\
+        expandedb u s'' B (Done s' B') b2 /\ b = b1 || b2.
   Proof.
+    move=>/[dup] /expandedb_same_structure.
+    case: C => //= A' B0' B' _.
     remember (And _ _ _) as g0 eqn:Hg0.
     remember (Done _ _) as s1 eqn:Hs1 => H.
-    elim: H A B0 B C Hg0 s' Hs1; clear => //.
-    - move=> s s' AB alt + A B0 B alt' ? s'' [] ??; subst.
+    elim: H A B0 B A' B0' B' Hg0 s' Hs1; clear => //.
+    - move=> s1 s2 A A' + B C0 C B' C0' C' ? s3 [??]; subst.
       move=> /simpl_expand_and_solved. 
-      move => [s' [A' [B']]] => -[H1 [H2 H3]]; subst.
+      move => [s' [Ax [Bx']]] => -[H1 [H2 [???]]]; subst.
       do 3 eexists; exists false, false; repeat split; apply: expanded_done; eassumption.
-    - move=> s s' r A B b + HB IH A1 B01 B1 C ? s2 ?; subst.
-      move=> /simpl_expand_and_cut [].
-        move=> [A'[HA']]?;subst.
-        have := IH _ _ _ _ erefl _ erefl.
-        move=> [s''[A2[B2[b1[b2 [HA1 HB2]]]]]].
-        (* move=> [s3 [A2 [B2 [[? HA1] HB2]]]]. *)
+    - move=> s1 s2 r A A' b + HB IH B C0 C B2 C0' C2 ? s3 ?; subst => /=.
+      case HA: expand => //=[s4 B1|s4 B1].
+        move=>[??]; subst.
+        have {IH} := IH _ _ _ _ _ _ erefl _ erefl.
+        move=> [s'[B3[C3[b1[b2[HB2[HC ?]]]]]]]; subst.
         do 5 eexists; repeat split.
-        - apply: expanded_cut HA' HA1.
-        - apply HB2.
+        - apply: expanded_cut HA HB2.
+        - apply HC.
         - reflexivity.
-      move=> [s'' [A' [B' [HA'[HB' ?]]]]]; subst.
-      have {IH} := IH _ _ _ _ erefl _ erefl.
-      move=> /= [s3 [A2 [B2 [b1[b2[EA2 [EB2 ?]]]]]]]; subst.
-      have [_ +]:= expand_solved_success HA'.
-      move=>/success_cut.
-      move=> scA1.
-      have[[??]?] := expanded_success scA1 EA2; subst.
+      case HB1':expand => //[s5 C1][??]; subst.
+      have {IH} := IH _ _ _ _ _ _ erefl _ erefl.
+      move=> /= [s5 [B1' [C1' [b1[b2[EA2 [EB2 ?]]]]]]]; subst.
+      have [[??]+]:= expand_solved_same _ HA; subst.
+      rewrite -success_cut => scA1.
+      have ?:= expand_cb_same_subst _ HB1'; subst.
+      have[[??]?] := expanded_success _ scA1 EA2; subst.
+      rename B1 into A1.
+      rename B2 into A2.
+      rename C into B.
+      rename C1 into B1.
+      rename C2 into B2.
       do 5 eexists; repeat split.
-      - apply: expanded_done HA'.
-      - apply: expanded_cut HB' EB2.
+      - apply: expanded_done HA.
+      - rewrite ges_subst_cutl in EB2.
+        apply: expanded_cut HB1' EB2.
       - reflexivity.
-    - move=> s1 s2 r ? D b + H IH A B0 B C ? s3 ?; subst.
+    - move=> s1 s2 r A A' b + HB IH B C0 C B2 C0' C2 ? s3 ?; subst.
       move=> /simpl_expand_and_expanded [].
-        move=> [A' [EA ?]];subst.
-        have:= IH _ _ _ _ erefl _ erefl.
-        move=> /= [s4 [A2 [B2 [b1[b2[EA2 [EB2 ?]]]]]]]; subst.
+        move=> [Ax [EA ?]];subst.
+        have:= IH _ _ _ _ _ _ erefl _ erefl.
+        move=> /= [s4 [A2 [B2' [b1[b2[EA2 [EB2 ?]]]]]]]; subst.
         do 5 eexists; repeat split => //=.
           apply: expanded_step EA EA2.
         apply: EB2.
-      move=> [s4 [A' [B' [EA' [EB' ?]]]]]; subst.
-      have:= IH _ _ _ _ erefl _ erefl.
-      move=> /= [s5 [A2 [B2 [b1[b2[EA2 [EB2 ?]]]]]]]; subst.
-      have [_ sA']:= expand_solved_success EA'.
-      have /= [[??]?] := expanded_success sA' EA2; subst.
-      subst.
+      move=> [s4 [A'' [B'' [EA' [EB' ?]]]]]; subst.
+      have:= IH _ _ _ _ _ _ erefl _ erefl.
+      move=> /= [s5 [A2' [B2' [b1[b2[EA2 [EB2 ?]]]]]]]; subst.
+      have [[??] sA']:= expand_solved_same _ EA'; subst.
+      have /= [[??]?] := expanded_success _ sA' EA2; subst.
       do 5 eexists; repeat split.
         apply: expanded_done EA'.
       apply: expanded_step EB' EB2.
   Qed.
 
   Lemma expand_success_done {A B0 s1 B s2 B' b}: 
-    success A -> expandedb s1 B (Done s2 B') b ->
-      expanded s1 (And A B0 B) 
+    success A -> expandedb u (get_substS s1 A) B (Done s2 B') b ->
+      expanded u s1 (And A B0 B) 
         (Done s2 (And (if b then cutl A else A) (if b then cutl B0 else B0) B')).
   Proof.
+    remember (get_substS _ _) as S eqn:HS.
     remember (Done _ _) as RD eqn:HRD => + H.
-    elim: H A B0 s2 B' HRD => //; clear.
-    - move=> s s' A A' H A0 B0 _ _ [<-<-] sA0.
+    elim: H A B0 s1 s2 B' HS HRD => //; clear.
+    - move=> s s' A A' H A0 B0 s1 _ _ ? [<-<-] sA0; subst.
+      have [[??]sA]:= expand_solved_same _ H; subst.
       exists false.
       apply: expanded_done.
-      rewrite /= (succes_is_solved _ sA0) H//.
-    - move=> s s' r A B b HA HB IH A0 B0 s2 C? sA0; subst.
+      rewrite /= succes_is_solved//.
+      rewrite (succes_is_solved)//=.
+    - move=> s s' r A B b HA HB IH A0 B0 s1 s2 C?? sA0; subst.
       exists true.
-      have [b1 {}IH]:= IH _ (cutl B0) _ _ erefl (success_cut sA0).
-      rewrite !cutl2 !if_same in IH.
-      apply: expanded_cut.
-      move=>/=; rewrite (succes_is_solved _ sA0) HA//.
-      apply: IH.
-    - move=> s s' r A B b HA HB IH A0 B0 s2 C ? sA0; subst.
-      have [b1 H]:= IH A0 B0 _ _ erefl sA0.
+      rewrite -success_cut in sA0.
+      have:= IH (cutl A0) (cutl B0) s1 s2 C.
+      rewrite ges_subst_cutl => /(_ erefl erefl sA0).
+      rewrite !cutl2 !if_same.
+      move=>[b1 {}IH].
+      rewrite success_cut in sA0.
+      apply: expanded_cut IH.
+      move=>/=; rewrite // (succes_is_solved _ _ sA0) HA//.
+    - move=> s s' r A B b HA HB IH A0 B0 s1 s2 C?? sA0; subst.
+      have [b1 H]:= IH A0 B0 _ _ _ erefl erefl sA0.
       eexists.
-      apply: expanded_step.
-        rewrite /= (succes_is_solved _ sA0) HA//.
-      apply H.
+      apply: expanded_step H.
+      rewrite /= (succes_is_solved _ _ sA0) HA//.
   Qed.
 
   (* This can be factored with the previous proof... *)
   Lemma expand_success_fail {A B0 s1 B B' b}: 
-    success A -> expandedb s1 B (Failed B') b ->
-      expandedb s1 (And A B0 B) 
+    success A -> expandedb u (get_substS s1 A) B (Failed B') b ->
+      expandedb u s1 (And A B0 B) 
         (Failed (And (if b then cutl A else A) (if b then cutl B0 else B0) B')) b.
   Proof.
+    remember (get_substS _ _) as S eqn:HS.
     remember (Failed _) as RD eqn:HRD => + H.
-    elim: H A B0 B' HRD => //; clear.
-    - move=> s A A' HA X B0 _ [<-] sX.
+    elim: H A B0 B' s1 HS HRD => //; clear.
+    - move=> s A A' HA B C0 C s1 ? [?] sB; subst.
       apply: expanded_fail.
-      rewrite /= (succes_is_solved _ sX) HA//.
-    - move=> s s' r A B b HA HB IH A0 B0 C? sA0; subst.
-      have {}IH := IH _ (cutl B0) _ erefl (success_cut sA0).
-      rewrite !cutl2 !if_same in IH.
-      apply: expanded_cut.
-      move=>/=; rewrite (succes_is_solved _ sA0) HA//.
-      apply: IH.
-    - move=> s s' r A B b HA HB IH A0 B0 C ? sA0; subst.
-      have {}IH := IH A0 B0 _ erefl sA0.
-      apply: expanded_step.
-        rewrite /= (succes_is_solved _ sA0) HA//.
-      apply IH.
+      rewrite /= (succes_is_solved _ _ sB) HA//.
+    - move=> s1 s2 r A A' b HA HA' IH B C0 C s3 ?? sB; subst.
+      rewrite -success_cut in sB.
+      have := IH _ _ _ s3 _ erefl sB.
+      rewrite ges_subst_cutl => /(_ (cutl C0) erefl).
+      rewrite !cutl2 !if_same => {}IH.
+      apply: expanded_cut IH.
+      rewrite success_cut in sB.
+      move=>/=; rewrite //= (succes_is_solved _ _ sB) HA//.
+    - move=> s1 s2 r A A' b HA HA' IH B C0 C s3 ?? sB; subst.
+      have := IH _ _ _ s3 _ erefl sB.
+      move => /(_ (C0) erefl) {}IH.
+      apply: expanded_step IH.
+      move=>/=; rewrite //= (succes_is_solved _ _ sB) HA//.
   Qed.
 
   Lemma expanded_and_correct {s0 s1 s2 A C B0 B D x} :
-      expanded s0 A (Done s1 B) -> expandedb s1 C (Done s2 D) x ->
-        expanded s0 (And A B0 C) 
+      expanded u s0 A (Done s1 B) -> expandedb u s1 C (Done s2 D) x ->
+        expanded u s0 (And A B0 C) 
           (Done s2 (And (if x then cutl B else B) (if x then cutl B0 else B0) D)).
   Proof.
     remember (Done _ _) as RD eqn:HRD => -[b H].
     elim: H s1 s2 C B0 B D HRD x => //=; clear.
     + move=> s1 s2 A B eA s3 s4 C D E F [??] b;subst.
-      have [??]:= expand_solved_same eA; subst.
-      have:= (expand_solved_success eA).1.
+      have [??]:= expand_solved_same _ eA; subst.
+      have [[??]]:= expand_solved_same _ eA; subst.
       apply: expand_success_done.
     + move=> s s' r A CA ? H H1 IH ?? ? B0 ?? /[subst1] b H2.
       have [b1 {}IH]:= IH _ _ _ B0 _ _ erefl _ H2.
@@ -310,20 +222,22 @@ Module RunP (A: Unif).
       by apply: IH.
   Qed.
 
-  Lemma expandes_and_fail {s A B0 B C}:
-    expanded s (And A B0 B) (Failed C) ->
-      (exists C', expanded s A (Failed C')) \/ (exists s' A' B', expanded s A (Done s' A') /\ expanded s' B (Failed B')).
+  (* Lemma expandes_and_fail {s A B0 B C}:
+    expanded u s (And A B0 B) (Failed C) ->
+      (exists C', expanded u s A (Failed C')) \/ 
+        (exists s' A' B', expanded u s A (Done s' A') /\ expanded u s B (Failed B')).
   Proof.
     remember (And _ _ _) as R eqn:HR.
     remember (Failed _) as F eqn:HF => -[b H].
     elim: H A B0 B C HR HF => //=; clear.
-    + move=> ??? + ???? ? [] ?;subst => /simpl_expand_and_fail [].
-        move=>[A'[HA' _]].
-        left; do 2 eexists; apply: expanded_fail HA'.
-      move=> [s'[A'[B'[HA'[HB' _]]]]].
+    + move=> s1 A A' + B C0 C _ ? _ /=; subst => /simpl_expand_and_fail [].
+        move=>[Ax[HAx _]].
+        left; do 2 eexists; apply: expanded_fail HAx.
+      move=> [s'[A2[B2[HA'[HB' ?]]]]]; subst.
+      have [[??]sA]:= expand_solved_same HA'; subst.
       right; do 3 eexists; split.
         eexists; apply: expanded_done HA'.
-      eexists; apply: expanded_fail HB'.
+      eexists; apply: expanded_fail. HB'.
     + move=> s s' r A B b + HB IH C D E F ??; subst.
       move=> /simpl_expand_and_cut[].
         move=>[A'[HA' ?]];subst.
@@ -363,11 +277,11 @@ Module RunP (A: Unif).
       do 3 eexists; split.
         eexists; apply: expanded_done H2.
       eexists; apply: expanded_step H3 H5.
-  Qed.
+  Qed. *)
 
   Lemma expanded_and_fail_left {s A B0 FA}:
-    expanded s A (Failed FA) ->
-      forall B, expanded s (And A B0 B) (Failed (And FA B0 B)).
+    expanded u s A (Failed FA) ->
+      forall B, expanded u s (And A B0 B) (Failed (And FA B0 B)).
   Proof.
     move=> [? H].
     remember (Failed _) as F eqn:HF.
@@ -388,16 +302,15 @@ Module RunP (A: Unif).
   Qed.
 
   Lemma run_and_fail_both {s s' A B B0 SA FB b}:
-    expanded s A (Done s' SA) -> expandedb s' B (Failed FB) b ->
-      expanded s (And A B0 B) (Failed (And (if b then cutl SA else SA) (if b then cutl B0 else B0) FB)).
+    expanded u s A (Done s' SA) -> expandedb u s' B (Failed FB) b ->
+      expanded u s (And A B0 B) (Failed (And (if b then cutl SA else SA) (if b then cutl B0 else B0) FB)).
   Proof.
     move=> [b1 H].
     remember (Done _ _) as D eqn:HD.
     elim: H B s' SA HD b => //=; clear.
     + move=> s1 s2 A B HA C s3 D [??] b H; subst.
-      eexists.
-      have H1:= expand_solved_same HA; rewrite 2!H1.
-      apply: expand_success_fail (expand_solved_success HA).2 H.
+      have [[??]sA]:= expand_solved_same _ HA; subst.
+      eexists; apply: expand_success_fail sA H.
     + move=> s s' r A B ? H H1 IH B1 s1 alt ? b H2; subst => //=.
       have [b1 H3] := IH _ _ _ erefl b H2.
       eexists;apply: expanded_cut => /=.
@@ -411,46 +324,47 @@ Module RunP (A: Unif).
   Qed.
 
   Lemma expanded_or_correct_left {s s' A A'} b:
-    expandedb s A (Done s' A') b ->
-      forall s2 B, expanded s (Or A s2 B) (Done s' (Or A' s2 (if b then cutr B else B))).
+    expandedb u s A (Done s' A') b ->
+      forall s2 B, expanded u s (Or A s2 B) (Done s' (Or A' s2 (if b then cutr B else B))).
   Proof.
     remember (Done _ _) as D eqn:HD => H.
     elim: H s' A' HD => //=; clear.
     + move=> s s' A A' HA s2 B [] ?? s3 C; subst.
       eexists; apply: expanded_done => //= ; rewrite HA.
       case: ifP => //H.
-      by rewrite (is_dead_expand H) in HA.
+      by rewrite (is_dead_expand _ H) in HA.
     + move=> s1 s2 r A B b HA HB IH s3 C ? s4 D /[subst].
       have /= [? {IH}]:= IH _ _ erefl s4 (cutr D).
       rewrite cutr2 if_same => IH.
       eexists; apply: expanded_step => //=.
         case: ifP => // dA.
-          by rewrite (is_dead_expand dA) in HA.
+          by rewrite (is_dead_expand _ dA) in HA.
         by rewrite HA.
       apply: IH.
     + move=> s1 s2 r A B b HA HB IH s' C ? s4 D /[subst].
       have [? {}IH] := IH _ _ erefl s4 D.
       eexists; apply: expanded_step => //=.
         case: ifP=> dA.
-          by rewrite (is_dead_expand dA) in HA.
+          by rewrite (is_dead_expand _ dA) in HA.
         by rewrite HA.
       apply IH. 
   Qed.
 
   Lemma expanded_or_complete {s s' s2 A A' B B' b}:
-    expandedb s (Or A s2 B) (Done s' (Or A' s2 B')) b ->
+    expandedb u s (Or A s2 B) (Done s' (Or A' s2 B')) b ->
       (is_dead A = false /\ 
-        exists b, expandedb s A (Done s' A') b /\ B' = if b then cutr B else B) \/ 
-        (is_dead A /\ A = A' /\ expanded s B (Done s' B')).
+        exists b, expandedb u s A (Done s' A') b /\ B' = if b then cutr B else B) \/ 
+        (is_dead A /\ A = A' /\ expanded u s2 B (Done s' B')).
   Proof.
     rewrite /expanded.
     remember (Done _ _) as RD eqn:HRD.
     remember (Or A _ _) as RO eqn:HRO => H.
     elim: H s' s2 A' B' A B HRO HRD => //=; clear.
-    + move=> s1 s3 C D + A B HRO ???? [] ??; subst.
+    + move=> s1 s3 A A' + s2 s4 B C D E ? [??]; subst.
       move=> /simpl_expand_or_solved [].
         move=> [A2 [HA']] [??];subst.
-        have dA := success_is_dead (expand_solved_success HA').1.
+        have [[??]sA] := expand_solved_same _ HA'; subst.
+        have dA := success_is_dead sA.
         left; repeat split => //.
         exists false; split => //; apply: expanded_done HA'.
       move=> [B' [dA [HB' [??]]]];subst.
@@ -470,7 +384,7 @@ Module RunP (A: Unif).
         right; repeat split; eexists; apply: expanded_cut eB H.
       case eA: expand => //[s1' A1'|s1' A1'][??]; subst; left; repeat split;
         have:= IH _ _ _ _ _ _ erefl erefl => -[][]; 
-        rewrite (expand_not_dead dA eA)// => _ [b [H1 H2]]; subst.
+        rewrite (expand_not_dead _ dA eA)// => _ [b [H1 H2]]; subst.
         eexists; split => //; apply: expanded_step eA H1.
       eexists; split.
         apply: expanded_cut eA H1.
@@ -479,8 +393,8 @@ Module RunP (A: Unif).
   
   Lemma expanded_or_correct_left_fail {s A A'} b:
     is_dead A = false ->
-    expandedb s A (Failed A') b ->
-      forall s2 B, expanded s (Or A s2 B) (Failed (Or A' s2 (if b then cutr B else B))).
+    expandedb u s A (Failed A') b ->
+      forall s2 B, expanded u s (Or A s2 B) (Failed (Or A' s2 (if b then cutr B else B))).
   Proof.
     remember (Failed _) as D eqn:HD => + H.
     elim: H A' HD => //=; clear.
@@ -488,12 +402,12 @@ Module RunP (A: Unif).
       eexists; apply: expanded_fail => /=.
       rewrite HA s3//.
     + move=> s1 s2 r A B b HA HB IH C ? dA s4 D /[subst].
-      have [? {}IH]:= IH _ erefl (expand_not_dead dA HA) s4 (cutr D).
+      have [? {}IH]:= IH _ erefl (expand_not_dead _ dA HA) s4 (cutr D).
       eexists; apply: expanded_step => //=.
         rewrite dA HA//.
       move: IH; rewrite cutr2 if_same => H; eassumption.
     + move=> s1 s2 r A B b HA HB IH C ? dA s4 D /[subst].
-      have [? {}IH] := IH _ erefl (expand_not_dead dA HA) s4 D.
+      have [? {}IH] := IH _ erefl (expand_not_dead _ dA HA) s4 D.
       eexists; apply: expanded_step => //=.
       rewrite dA.
         by rewrite HA.
@@ -501,8 +415,8 @@ Module RunP (A: Unif).
   Qed.
 
   Lemma run_or_correct_left {s1 A s2 A' b sB B}:
-    runb s1 A s2 A' b ->
-      run s1 (Or A sB B) s2 (Or A' sB (if b then cutr B else B)).
+    runb u s1 A s2 A' b ->
+      run u s1 (Or A sB B) s2 (Or A' sB (if b then cutr B else B)).
   Proof.
     move => H.
     elim: H sB B => //; clear.
@@ -510,15 +424,15 @@ Module RunP (A: Unif).
       have [? H1]:= expanded_or_correct_left _ H s2 A'.
       eexists.
       apply: run_done H1 _.
-      have sB := expanded_Done_success H.
+      have sB := expanded_Done_success _ H.
       move=>/=.
       rewrite success_is_dead//.
     + move=> s s' r A B C D b1 b2 b3 HE HN HR IH ? s2 E;subst.
       case dA: (is_dead A).
-        have H := is_dead_expanded s dA.
-        have [[?]?] := expanded_consistent H HE; subst.
+        have H := is_dead_expanded _ s dA.
+        have [[?]?] := expanded_consistent (H _) HE; subst.
         by rewrite (is_dead_next_alt dA) in HN.
-      have /= dB := expanded_not_dead dA HE.
+      have /= dB := expanded_not_dead _ dA HE.
       have [b3 H] := expanded_or_correct_left_fail _ dA HE s2 E.
       (* have {}HN: next_alt s (Or B s2 (if b1 then cutr E else E)) = Some (s', Or C s2 (if b1 then cutr E else E)).
         move=>/=; rewrite ((next_alt_dead HN)) HN//. *)
@@ -534,16 +448,27 @@ Module RunP (A: Unif).
       apply: IH1.
   Qed.
 
+  Lemma is_dead_runb {s1 s2 A B b}: is_dead A -> runb u s1 A s2 B b -> False.
+  Proof.
+    move=> +H.
+    elim: H; clear.
+    - move=> s s' A B C b /expandedb_Done_not_failed ++ /is_dead_failed; congruence.
+    - move=> s1 s2 s3 A B C D b1 b2 b3 +++++ H; move:H.
+      move=>/[dup]dA/is_dead_expanded- /(_ _ s1).
+      move=> /[dup]H1/(_ u) /expanded_consistent H {}/H[][??]; subst.
+      rewrite (is_dead_next_alt dA)//.
+  Qed.
+
   Lemma run_or_complete {s1 s2 A B SOL altAB}:
-    run s1 (Or A s2 B) SOL altAB ->
-      (exists altA, run s1 A SOL altA) \/ 
-        (exists altB, run s2 B SOL altB).
+    run u s1 (Or A s2 B) SOL altAB ->
+      (exists altA, run u s1 A SOL altA) \/ 
+        (exists altB, run u s2 B SOL altB).
   Proof.
     remember (Or _ _ _) as O1 eqn:HO1.
     move=> [b H].
     elim: H s2 A B HO1 => //=; clear.
     + move=> s st s' alt C b H ? s2 D E ?; subst.
-      have /= := expandedb_same_structure H.
+      have /= := expandedb_same_structure _ H.
       case: alt H => //= D' s2' E' H /and3P[/eqP? _ _]; subst.
       have:= expanded_or_complete H.
       move=> [][dD].
@@ -552,17 +477,17 @@ Module RunP (A: Unif).
         eexists (clean_success D'), _.
         apply: run_done H1 erefl.
       move=> [?[H1]] H2; subst.
-      admit.
+      right.
+      do 2 eexists.
+      apply: run_done H2 erefl.
     + move=> s s1 s2 A B C D b1 b2 b3 H1 H2 H3 IH ? s4 E F ?; subst.
-      have /= := expandedb_same_structure H1.
+      have /= := expandedb_same_structure _ H1.
       case: B H1 H2 => //= D' s2' E' H1 + /and3P[/eqP? _ _]; subst.
       case: ifP => dD'.
         case X: next_alt => //=[[s4 E2]][??]; subst.
         have [[x [b {}IH]]|[x [b{}IH]]] := IH _ _ _ erefl.
-          admit.
-        left; do 2 eexists.
-        apply: run_backtrack _ _ IH erefl.
-        admit.
+          by have:= is_dead_runb dD' IH.
+        Search expandedb u Failed Or.
         admit.
       case X: next_alt => //=[[s4 E2]|].
         move=> [??]; subst.
@@ -572,13 +497,13 @@ Module RunP (A: Unif).
       case: ifP => //dE.
       case Y: next_alt => //=[[s4 E2]][??]; subst.
       have [[x [b {}IH]]|[x [b{}IH]]] := IH _ _ _ erefl.
-        admit.
+        by have:= is_dead_runb is_dead_dead IH.
       admit.
   Abort.
 
   (*   Lemma run_or_fail {s1 s2 A B b}:
-    run s1 (Or A s2 B) Failed ->
-      run s1 A Failed /\ (run_classic s1 A b -> run s2 B Failed).
+    run u s1 (Or A s2 B) Failed ->
+      run u s1 A Failed /\ (run_classic u s1 A b -> run u s2 B Failed).
   Proof.
     move=> H.
     remember (Or _ _ _) as O eqn:HO.
@@ -610,8 +535,8 @@ Module RunP (A: Unif).
   Qed.
 
   Lemma run_Failed_cut {s s2 A B}:
-    run s A Failed ->
-      run s (Or A s2 (cutl B)) Failed.
+    run u s A Failed ->
+      run u s (Or A s2 (cutl B)) Failed.
   Proof.
     remember Failed as F eqn:HF.
     move=> H.
@@ -629,10 +554,10 @@ Module RunP (A: Unif).
   Qed.
 
   Lemma run_or_fail1 {s1 s2 g1 g2}:
-      run s1 g1 Failed -> (run_classic s1 g1 Failed -> run s2 g2 Failed) ->
-        run s1 (Or g1 s2 g2) Failed.
+      run u s1 g1 Failed -> (run_classic u s1 g1 Failed -> run u s2 g2 Failed) ->
+        run u s1 (Or g1 s2 g2) Failed.
   Proof.
-    move: (classic (run_classic s1 g1 Failed)) => [].
+    move: (classic (run_classic u s1 g1 Failed)) => [].
     + move=> H + /(_ H) => H1; move: H.  
       remember Failed as F eqn:HF.
       elim: H1 s2 g2 HF; clear => //=.
@@ -672,18 +597,11 @@ Module RunP (A: Unif).
   Qed.
 
   Lemma run_or_fail2 {s1 s2 g1 g2 g3}:
-      run s1 g1 Failed -> expand s1 g1 = CutBrothers g3 -> (* g1 coulbe not an immediate cutl, but expand... to a cutl *)
-        run s1 (Or g1 s2 g2) Failed.
+      run u s1 g1 Failed -> expand u s1 g1 = CutBrothers g3 -> (* g1 coulbe not an immediate cutl, but expand u... to a cutl *)
+        run u s1 (Or g1 s2 g2) Failed.
   Proof.
     move=> H H1; apply: run_or_fail1 H _ => H2.
     inversion H2; subst; congruence.
   Qed.  *)
 
-  Lemma expandedb_failed {s1 A B b1}: expandedb s1 A (Failed B) b1 -> failed B.
-  Proof.
-    remember (Failed B) as fB eqn:HfB => H.
-    elim: H B HfB => //; clear.
-    move=> s1 A B H C []<-.
-    have []:= expand_failure_failed H => //.
-  Qed.
 End RunP.
